TheoryTask/qcp-binary-democases/SeparationLogic/examples/sll_project_proof_auto.v
@@ -67,6 +67,12 @@ Proof. Admitted.
 Lemma proof_of_cons_list_box_safety_wit_2 : cons_list_box_safety_wit_2.
 Proof. Admitted. 
 
+Lemma proof_of_cons_list_box_safety_wit_3 : cons_list_box_safety_wit_3.
+Proof. Admitted. 
+
+Lemma proof_of_cons_list_box_safety_wit_4 : cons_list_box_safety_wit_4.
+Proof. Admitted. 
+
 Lemma proof_of_cons_list_box_partial_solve_wit_1 : cons_list_box_partial_solve_wit_1.
 Proof. Admitted. 
 
@@ -83,6 +89,12 @@ Lemma proof_of_map_list_box_partial_solve_wit_1 : map_list_box_partial_solve_wit
 Proof. Admitted. 
 
 Lemma proof_of_map_list_box_partial_solve_wit_2 : map_list_box_partial_solve_wit_2.
+Proof. Admitted. 
+
+Lemma proof_of_map_list_box_partial_solve_wit_3 : map_list_box_partial_solve_wit_3.
+Proof. Admitted. 
+
+Lemma proof_of_map_list_box_partial_solve_wit_4 : map_list_box_partial_solve_wit_4.
 Proof. Admitted. 
 
 Lemma proof_of_free_list_box_return_wit_1 : free_list_box_return_wit_1.
@@ -148,9 +160,18 @@ Proof. Admitted.
 Lemma proof_of_sllb2array_partial_solve_wit_1 : sllb2array_partial_solve_wit_1.
 Proof. Admitted. 
 
-Lemma proof_of_sllb2array_partial_solve_wit_2_pure : sllb2array_partial_solve_wit_2_pure.
+Lemma proof_of_sllb2array_partial_solve_wit_2 : sllb2array_partial_solve_wit_2.
 Proof. Admitted. 
 
-Lemma proof_of_sllb2array_partial_solve_wit_2 : sllb2array_partial_solve_wit_2.
+Lemma proof_of_sllb2array_partial_solve_wit_3_pure : sllb2array_partial_solve_wit_3_pure.
+Proof. Admitted. 
+
+Lemma proof_of_sllb2array_partial_solve_wit_3 : sllb2array_partial_solve_wit_3.
+Proof. Admitted. 
+
+Lemma proof_of_sllb2array_partial_solve_wit_4_pure : sllb2array_partial_solve_wit_4_pure.
+Proof. Admitted. 
+
+Lemma proof_of_sllb2array_partial_solve_wit_4 : sllb2array_partial_solve_wit_4.
 Proof. Admitted. 
 
