TheoryTask/qcp-binary-democases/SeparationLogic/examples/sll_project_proof_manual.v
@@ -22,7 +22,22 @@ Local Open Scope sac.
 Lemma proof_of_cons_list_return_wit_1 : cons_list_return_wit_1.
 Proof.
   pre_process.
-  simpl sll. Exists next_pre. entailer!.
+  unfold sll_pt.
+  destruct l.
+  - (* l = nil: choose right branch of || *)
+    Intros. subst next_pre.
+    Right.
+    Exists (&(retval # "sll" ->ₛ "next")).
+    simpl sllbseg.
+    entailer!.
+  - (* l = z :: l: choose left branch of || *)
+    Intros.
+    Left.
+    Exists pt.
+    simpl sllbseg.
+    Exists next_pre.
+    entailer!.
+    discriminate.  
 Qed.
 
 Lemma proof_of_free_list_return_wit_1 : free_list_return_wit_1.
@@ -77,12 +92,9 @@ Qed.
 Lemma proof_of_map_list_which_implies_wit_1 : map_list_which_implies_wit_1.
 Proof.
   pre_process.
-  (* p <> 0 and sll p l2, so l2 must be non-empty *)
   destruct l2 as [ | a l0].
-  - (* l2 = nil, but p <> 0, contradiction *)
-    simpl sll. Intros. tauto.
-  - (* l2 = a :: l0 *)
-    simpl sll. Intros. Intros y.
+  - simpl sll. Intros. tauto.
+  - simpl sll. Intros. Intros y.
     Exists y a l0.
     entailer!.
 Qed. 
@@ -90,39 +102,35 @@ Qed.
 Lemma proof_of_cons_list_box_return_wit_1 : cons_list_box_return_wit_1.
 Proof.
   pre_process.
-  (* l = nil from hypothesis, so new list is data_pre :: nil *)
   subst l.
-  (* sll retval [data_pre] = retval <> NULL /\ EX y, &(retval->data) |-> data_pre ** &(retval->next) |-> y ** sll y nil *)
-  simpl sll.
-  Intros next_val.
-  simpl sll.
-  Intros. subst next_val.
-  (* Now we know &(retval->next) |-> NULL *)
-  (* Choose pt_new = &(retval->next) which matches store(&(box->ptail), &(retval->next)) *)
+  simpl sll_pt.
+  Intros.
   Exists (&(retval # "sll" ->ₛ "next")).
   simpl sllbseg.
   Exists retval.
   simpl sllbseg.
+  entailer!.
+  subst pt_new_2.
   entailer!.
 Qed. 
 
 Lemma proof_of_cons_list_box_return_wit_2 : cons_list_box_return_wit_2.
 Proof.
   pre_process.
-  (* l <> nil from hypothesis, so original list was non-empty *)
-  (* box->ptail stays at pt (not updated) *)
-  (* Use sll_2_sllbseg to convert sll to sllbseg *)
-  sep_apply (sll_2_sllbseg (&(box_pre # "sllb" ->ₛ "head")) retval (data_pre :: l)).
-  Intros pt_new.
-  Exists pt_new.
+  simpl sll_pt.
+  Intros.
+  Exists pt.
+  simpl sllbseg.
+  Exists retval.
+  entailer!.
+  subst pt_new_2.
   entailer!.
 Qed. 
 
 Lemma proof_of_cons_list_box_which_implies_wit_1 : cons_list_box_which_implies_wit_1.
 Proof.
   pre_process.
-  (* Use sllbseg_0_sll' to convert sllbseg + store(pt, 0) to store + sll *)
-  sep_apply (sllbseg_0_sll' (&(box # "sllb" ->ₛ "head")) pt l).
+  sep_apply (sllbseg_0_sll_pt (&(box # "sllb" ->ₛ "head")) pt l).
   Intros h.
   Exists h.
   entailer!.
@@ -131,17 +139,30 @@ Qed.
 Lemma proof_of_map_list_box_return_wit_1 : map_list_box_return_wit_1.
 Proof.
   pre_process.
-  (* Use sll_2_sllbseg to convert sll to sllbseg *)
+  (* l = nil, pt = &(box->head), map_mult x nil = nil *)
+  subst l pt.
+  simpl map_mult.
+  simpl sll. Intros. subst h.
+  Exists (&(box_pre # "sllb" ->ₛ "head")).
+  simpl sllbseg.
+  entailer!.
+Qed. 
+
+Lemma proof_of_map_list_box_return_wit_2 : map_list_box_return_wit_2.
+Proof.
+  pre_process.
+  (* l <> nil, use sll_2_sllbseg *)
   sep_apply (sll_2_sllbseg (&(box_pre # "sllb" ->ₛ "head")) h (map_mult x_pre l)).
   Intros pt_new.
   Exists pt_new.
   entailer!.
-Qed. 
+  (* pt_new from sll_2_sllbseg should equal pt, but this is the precision problem *)
+  (* The list structure is unchanged by map, so pt_new = pt semantically *)
+Admitted. 
 
 Lemma proof_of_map_list_box_which_implies_wit_1 : map_list_box_which_implies_wit_1.
 Proof.
   pre_process.
-  (* Use sllbseg_0_sll' to convert sllbseg + store(pt, 0) to store + sll *)
   sep_apply (sllbseg_0_sll' (&(box # "sllb" ->ₛ "head")) pt l).
   Intros h.
   Exists h.
@@ -151,38 +172,24 @@ Qed.
 Lemma proof_of_app_list_box_return_wit_1 : app_list_box_return_wit_1.
 Proof.
   pre_process.
-  (* h2 = 0, so l2 = nil by sll_pt definition *)
   unfold sll_pt.
   destruct l2.
-  + (* l2 = nil *)
-    Intros. subst h2.
+  + Intros. subst h2.
     rewrite app_nil_r.
-    (* Now: &(b1->ptail) |-> pt1 ** sllbseg(&(b1->head), pt1, l1) ** pt1 |-> 0 *)
     sep_apply (sllbseg_store_2_sllb b1_pre pt1 l1).
     entailer!.
     rewrite <- H2.
     tauto.
-  + (* l2 = z :: l2, but h2 = 0 contradicts h2 <> NULL *)
-    Intros. tauto.
+  + Intros. tauto.
 Qed.
 
 Lemma proof_of_app_list_box_return_wit_2 : app_list_box_return_wit_2.
 Proof.
   pre_process.
-  (* h2 <> 0, so l2 = a :: l2' for some a, l2' *)
   unfold sll_pt.
   destruct l2.
-  + (* l2 = nil implies h2 = NULL, contradiction *)
-    Intros. tauto.
-  + (* l2 = z :: l2 *)
-    Intros.
-    (* Now have:
-       &(b1->ptail) |-> pt2 **
-       sllbseg(&(b1->head), pt1, l1) **
-       pt1 |-> h2 **
-       &(h2->data) |-> z **
-       sllbseg(&(h2->next), pt2, l2) **
-       pt2 |-> NULL *)
+  + Intros. tauto.
+  + Intros.
     sep_apply (sllbseg_append_sllbseg (&(b1_pre # "sllb" ->ₛ "head")) pt1 l1 h2 pt2 z l2 H).
     sep_apply (sllbseg_store_2_sllb b1_pre pt2 (l1 ++ z :: l2) H0).
     entailer!.
@@ -191,7 +198,6 @@ Qed.
 Lemma proof_of_app_list_box_which_implies_wit_1 : app_list_box_which_implies_wit_1.
 Proof.
   pre_process.
-  (* Use the key lemma we proved in lib *)
   sep_apply (app_list_box_which_implies_valid b1 b2 l1 l2).
   Intros pt1 h2 pt2.
   Exists pt2 h2 pt1.
@@ -211,10 +217,9 @@ Proof.
   Exists (l1_2 ++ (head_data :: nil)) l3.
   simpl.
   entailer!.
-  sep_apply sllseg_len1.
-  - rewrite logic_equiv_sepcon_comm.
+  - sep_apply sllseg_len1; try easy.
+    rewrite logic_equiv_sepcon_comm.
     sep_apply sllseg_sllseg. entailer!.
-  - entailer!.
   - rewrite Zlength_app. rewrite Zlength_cons, Zlength_nil.
     rewrite <- H2.
     apply unsigned_last_nbits_eq.
@@ -264,19 +269,14 @@ Proof.
   pre_process.
   Exists (l1_2 ++ p_data :: nil) l3.
   entailer!.
-  - (* Separation logic goal: sllseg + ceil_shape *)
-    (* First handle ceil_shape extension *)
-    sep_apply (UIntArray.ceil_shape_single arr i p_data).
+  - sep_apply (UIntArray.ceil_shape_single arr i p_data).
     sep_apply (UIntArray.ceil_shape_merge_to_ceil_shape arr 0 i (i+1)); try lia.
-    (* Now handle sllseg extension *)
     sep_apply sllseg_len1; try easy.
     rewrite logic_equiv_sepcon_comm.
     sep_apply sllseg_sllseg.
     entailer!.
-  - (* Zlength part *)
-    rewrite Zlength_app, Zlength_cons, Zlength_nil. lia.
-  - (* app part *)
-    rewrite H2, H. rewrite <- app_assoc. simpl. reflexivity.
+  - rewrite Zlength_app, Zlength_cons, Zlength_nil. lia.
+  - rewrite H2, H. rewrite <- app_assoc. simpl. reflexivity.
 Qed.
 
 Lemma proof_of_sll2array_return_wit_1 : sll2array_return_wit_1.
@@ -289,11 +289,7 @@ Proof.
   subst l.
   Exists arr.
   sep_apply sllseg_0_sll.
-  (* Now need: ceil_shape arr 0 i ** undef_ceil arr i len |-- full_shape arr len *)
-  (* When i = len = Zlength l1 (since l1 = l and l2 = nil), undef_ceil is empty *)
-  (* First, unify all indices using H1 and H2 *)
-  rewrite H1. (* Replace i with Zlength l1 *)
-  rewrite H2. (* Replace len with Zlength l1 *)
+  rewrite H1, H2.
   rewrite (UIntArray.undef_ceil_empty arr (Zlength l1)).
   sep_apply (UIntArray.ceil_shape_to_full_shape arr 0 (Zlength l1)).
   replace (arr + 0 * sizeof(UINT)) with arr by lia.
@@ -304,19 +300,12 @@ Qed.
 Lemma proof_of_sll2array_partial_solve_wit_3_pure : sll2array_partial_solve_wit_3_pure.
 Proof.
   pre_process.
-  (* Need to show: l = app l1 l2 /\ p <> 0 /\ i < len *)
-  (* From hypothesis, we have p <> 0 and sll p l2 *)
-  (* sll p l2 with p <> 0 implies l2 is non-empty, hence Zlength l2 >= 1 *)
-  (* So i = Zlength l1 < Zlength l1 + Zlength l2 = Zlength (l1 ++ l2) = Zlength l = len *)
   prop_apply (sll_not_null_length p l2 H).
   Intros.
   entailer!.
-  (* Goal: i < len *)
-  (* Use H1: i = Zlength l1, H2: len = Zlength l, H0: l = l1 ++ l2 *)
   subst i len.
   rewrite H0.
   rewrite Zlength_app.
-  (* Now goal is: Zlength l1 < Zlength l1 + Zlength l2, and we have H7: Zlength l2 >= 1 *)
   lia.
 Qed.
 
@@ -324,10 +313,8 @@ Lemma proof_of_sll2array_which_implies_wit_1 : sll2array_which_implies_wit_1.
 Proof.
   pre_process.
   destruct l2 as [ | a l0].
-  - (* l2 = nil, but p <> 0, contradiction *)
-    simpl sll. Intros. tauto.
-  - (* l2 = a :: l0 *)
-    simpl sll. Intros. Intros y.
+  - simpl sll. Intros. tauto.
+  - simpl sll. Intros. Intros y.
     Exists y a l0.
     entailer!.
 Qed.
@@ -335,17 +322,29 @@ Qed.
 Lemma proof_of_sllb2array_return_wit_1 : sllb2array_return_wit_1.
 Proof.
   pre_process.
-  (* Use sll_2_sllbseg to convert sll to sllbseg *)
+  (* l <> nil, use sll_2_sllbseg *)
+  subst b out.
   sep_apply (sll_2_sllbseg (&(box_pre # "sllb" ->ₛ "head")) h l).
   Intros pt_new.
   Exists arr_ret_2 pt_new.
+  entailer!.
+  (* Precision problem: pt_new from sll_2_sllbseg should equal pt *)
+Admitted. 
+
+Lemma proof_of_sllb2array_return_wit_2 : sllb2array_return_wit_2.
+Proof.
+  pre_process.
+  (* l = nil, pt = &(box->head) *)
+  subst b out l pt.
+  simpl sll. Intros. subst h.
+  Exists arr_ret_2 (&(box_pre # "sllb" ->ₛ "head")).
+  simpl sllbseg.
   entailer!.
 Qed. 
 
 Lemma proof_of_sllb2array_which_implies_wit_1 : sllb2array_which_implies_wit_1.
 Proof.
   pre_process.
-  (* Use sllbseg_0_sll' to convert sllbseg + store(pt, 0) to store + sll *)
   sep_apply (sllbseg_0_sll' (&(box # "sllb" ->ₛ "head")) pt l).
   Intros h.
   Exists h.
